#### 1.5
##### 2.
###### （1）$P \rightarrow (Q \rightarrow R)$，$P \wedge Q \Rightarrow R$

证明：  
$1)\;P\wedge Q\Rightarrow P,\;Q$  
$2)\;P,\;P\to(Q\to R)\Rightarrow Q\to R$  
$3)\;Q,\;Q\to R\Rightarrow R$  
因此命题得证。  
<p align="right" style="font-size: 0.8em;">∎</p>

###### （3）$(P \rightarrow Q) \wedge (P \rightarrow R)$，$\neg(Q \wedge R)$，$S \lor P \Rightarrow S$

证明：  
$1)\;(P\to Q)\land(P\to R)\Rightarrow P\to Q,\;P\to R$  
$2)\;P\to Q,\;P\to R\Rightarrow P\to(Q\land R)$  
$3)\;P\to(Q\land R),\;\neg(Q\land R)\Rightarrow \neg P$  
$4)\;S\lor P,\;\neg P\Rightarrow S$  
因此命题得证。  
<p align="right" style="font-size: 0.8em;">∎</p>



#### 2. 用附加前提法证明
##### 1.
###### （1）$\neg P\lor Q,\;\neg Q\lor R,\;R\to S \Rightarrow P\to S$

LHS等价变换: 
$\neg P\lor Q\;\Leftrightarrow\;P\to Q,\qquad \neg Q\lor R\;\Leftrightarrow\;Q\to R$

附加前提 $P$：  
$1)\;P,\;P\to Q\Rightarrow Q$  
$2)\;Q,\;Q\to R\Rightarrow R$  
$3)\;R,\;R\to S\Rightarrow S$  
解除前提得 $P\to S$。  
<p align="right" style="font-size: 0.8em;">∎</p>

###### （4）$P\to(Q\to R),\;Q\to(R\to S)\Rightarrow P\to(Q\to S)$

附加前提 $P$：  
$1)\;P,\;P\to(Q\to R)\Rightarrow Q\to R$  
再附加前提 $Q$：  
$2)\;Q,\;Q\to R\Rightarrow R$  
$3)\;Q,\;Q\to(R\to S)\Rightarrow R\to S$  
$4)\;R,\;R\to S\Rightarrow S$  
解除 $Q$ 得 $Q\to S$，再解除 $P$ 得 $P\to(Q\to S)$。  
<p align="right" style="font-size: 0.8em;">∎</p>



#### 3. 用反证法证明
##### 1.
###### （1）$P\to \neg Q,\;Q\lor \neg R,\;R\wedge \neg S \Rightarrow \neg P$

证明：设 $P$。  
由 $R\wedge\neg S\Rightarrow R$，与 $Q\lor\neg R$ 得 $\neg R$ 为假，故 $Q$ 为真。  
又 $P\to\neg Q$ 与 $P$ 推出 $\neg Q$，与 $Q$ 矛盾。  
故设 $P$ 不成立，结论 $\neg P$。  
<p align="right" style="font-size: 0.8em;">∎</p>

###### （2）$P\lor Q,\;P\to R,\;Q\to S \Rightarrow R\lor S$

证明：设 $\neg(R\lor S)$，即 $\neg R\land \neg S$。  
由 $\neg R$ 与 $P\to R$ 得 $\neg P$；由 $\neg S$ 与 $Q\to S$ 得 $\neg Q$。  
与 $P\lor Q$ 矛盾，故 $\neg(R\lor S)$ 不成立，从而 $R\lor S$ 成立。  
<p align="right" style="font-size: 0.8em;">∎</p>
